spec+proof: fix domain schedule wrap
- Before this commit, domain_set_start would correctly set a new start
  index for the domain schedule, and would end the current domain, but
  would not end the entire current domain schedule to actually start
  the new schedule.

  Reserve the last index in the domain schedule to be an end marker. In
  domain_set_start set the current domain index to the second to last
  index, such that after index increment in next_domain, we hit the end
  marker and therefore start the new schedule.

- This change means that the valid_domain_list invariant now also
  depends on domain_index, which in turn means we need to prove more
  preservation lemmas. Use the infrastructure for domain field
  preservation from the InfoFlow session (PasUpdates.thy) in AInvs to
  reduce the number of lemma statements for this and re-use the setup
  in InfoFlow.

Signed-off-by: Gerwin Klein <gerwin.klein@proofcraft.systems>

spec/haskell/src/SEL4/Object/Domain.hs
@@ -43,9 +43,16 @@ domainScheduleConfigure :: Int -> Domain -> DomainDuration -> Kernel ()
 domainScheduleConfigure index domain duration =
     modify (\s -> s { ksDomSchedule = listUpdate (ksDomSchedule s) index (domain, duration) })
 
+domainSetStart :: Int -> Kernel ()
 domainSetStart start = do
+    -- order of modify calls matches C assignemtns
     modify (\s -> s { ksDomScheduleStart = start })
     modify (\s -> s { ksDomainTime = 0 })
+    -- set the index such that after increment in nextDomain, it will point to
+    -- the last domain schedule item, which is reserved to be an end marker.
+    schedule <- gets ksDomSchedule
+    before_end_index <- return $ length schedule - 2
+    modify (\s -> s { ksDomScheduleIdx = before_end_index })
     rescheduleRequired
 
 invokeDomain :: DomainInvocation -> Kernel ()
@@ -79,7 +86,7 @@ decodeDomainConfigure args extraCaps = do
     domain <- return $ args !! 1
     duration <- return $ parseTimeArg 2 args
     sched <- withoutFailure $ gets ksDomSchedule
-    when (index >= length sched) $ throw $ RangeError 0 (fromIntegral (length sched - 1))
+    when (index >= length sched - 1) $ throw $ RangeError 0 (fromIntegral (length sched - 2))
     when (fromIntegral domain >= numDomains)  $ throw $ RangeError 0 (fromIntegral (numDomains - 1))
     when (duration > maxDomainDuration) $ throw $ InvalidArgument 2
     when (duration == 0 && domain /= 0) $ throw $ InvalidArgument 1
