proof/invariant-abstract/DetSchedDomainTime_AI.thy
@@ -14,292 +14,200 @@ text \<open>
 \<close>
 
 (* Note: domains in the domain list should also be \<le> maxDomain, but this is not needed right now *)
-definition
-  "valid_domain_list_2 start dlist \<equiv>
-     0 < length dlist \<and> (\<forall>(d,time) \<in> set dlist. time = 0 \<longrightarrow> d = 0) \<and>
-     start < length dlist \<and> dlist ! start \<noteq> (0,0)"
+definition valid_domain_list_2 :: "nat \<Rightarrow> nat \<Rightarrow> (domain \<times> domain_duration) list \<Rightarrow> bool" where
+  "valid_domain_list_2 start index dlist \<equiv>
+     \<comment> \<open>We need at least two entries in the schedule: One active entry and the reserved domain end
+         marker at the end. Technically this is redundant with the last conjunct in this predicate,
+         but it is convenient to have it spelled out.\<close>
+     1 < length dlist \<and>
+     \<comment> \<open>Time can only be 0 in the end marker.\<close>
+     (\<forall>(d,time) \<in> set dlist. time = 0 \<longrightarrow> d = 0) \<and>
+     start < length dlist \<and>
+     \<comment> \<open>The start must always be a non-end-marker so that the schedule can make progress.\<close>
+     dlist ! start \<noteq> (0,0) \<and>
+     \<comment> \<open>The last entry in the schedule is reserved to always be an end marker.\<close>
+     dlist ! (length dlist - 1) = (0,0) \<and>
+     \<comment> \<open>The current index never gets to the final end marker.\<close>
+     index < length dlist - 1"
 
 abbreviation
   valid_domain_list :: "'z state \<Rightarrow> bool"
 where
-  "valid_domain_list \<equiv> \<lambda>s. valid_domain_list_2 (domain_start_index s) (domain_list s)"
+  "valid_domain_list \<equiv>
+     \<lambda>s. valid_domain_list_2 (domain_start_index s) (domain_index s) (domain_list s)"
 
 lemmas valid_domain_list_def = valid_domain_list_2_def
 
 lemma valid_domain_list_lift:
   assumes "\<And>P. f \<lbrace>\<lambda>s. P (domain_list s)\<rbrace>"
+  assumes "\<And>P. f \<lbrace>\<lambda>s. P (domain_index s)\<rbrace>"
   assumes "\<And>P. f \<lbrace>\<lambda>s. P (domain_start_index s)\<rbrace>"
   shows "f \<lbrace>valid_domain_list\<rbrace>"
-  by (rule hoare_lift_Pf[OF assms])
+  by (wp_pre, wps assms, wp)
 
 section \<open>Preservation of domain list validity\<close>
 
-(*
-  FIXME: cleanup
-  Many of these could be factored out into the general state_ext class instead, but they will be
-  applied to det_ext lemmas that contain e.g. preemption_point which needs the det_ext work_units,
-  i.e. those will need additional locales, because 'state_ext needs to be interpreted first
-  into ?'state_ext.
-*)
+abbreviation (input) domain_fields ::
+  "(ticks \<Rightarrow> nat \<Rightarrow> nat \<Rightarrow> (domain \<times> domain_duration) list \<Rightarrow> bool) \<Rightarrow> det_state \<Rightarrow> bool"
+  where
+  "domain_fields P s \<equiv> P (domain_time s) (domain_index s) (domain_start_index s) (domain_list s)"
+
+abbreviation (input) dlist_fields ::
+  "(nat \<Rightarrow> nat \<Rightarrow> (domain \<times> domain_duration) list \<Rightarrow> bool) \<Rightarrow> det_state \<Rightarrow> bool"
+  where
+  "dlist_fields P s \<equiv> P (domain_index s) (domain_start_index s) (domain_list s)"
+
+lemma valid_domain_list_lift':
+  assumes "\<And>P. f \<lbrace>domain_fields P\<rbrace>"
+  shows "f \<lbrace>valid_domain_list\<rbrace>"
+  by (wp assms)
+
 locale DetSchedDomainTime_AI =
-  assumes finalise_cap_domain_list_inv'[wp]:
-    "\<And>P cap fin. arch_finalise_cap cap fin \<lbrace>\<lambda>s::det_state. P (domain_list s)\<rbrace>"
-  assumes finalise_cap_domain_start_index_inv'[wp]:
-    "\<And>P cap fin. arch_finalise_cap cap fin \<lbrace>\<lambda>s::det_state. P (domain_start_index s)\<rbrace>"
-  assumes arch_activate_idle_thread_domain_list_inv'[wp]:
-    "\<And>P t. \<lbrace>\<lambda>s::det_state. P (domain_list s)\<rbrace> arch_activate_idle_thread t \<lbrace>\<lambda>_ s. P (domain_list s)\<rbrace>"
-  assumes arch_activate_idle_thread_domain_start_index_inv'[wp]:
-    "\<And>P t. arch_activate_idle_thread t \<lbrace>\<lambda>s::det_state. P (domain_start_index s)\<rbrace>"
-  assumes arch_switch_to_thread_domain_list_inv'[wp]:
-    "\<And>P t. \<lbrace>\<lambda>s::det_state. P (domain_list s)\<rbrace> arch_switch_to_thread t \<lbrace>\<lambda>_ s. P (domain_list s)\<rbrace>"
-  assumes arch_switch_to_thread_domain_start_index_inv'[wp]:
-    "\<And>P t. arch_switch_to_thread t \<lbrace>\<lambda>s::det_state. P (domain_start_index s)\<rbrace>"
-  assumes arch_get_sanitise_register_info_domain_list_inv'[wp]:
-    "\<And>P t. \<lbrace>\<lambda>s::det_state. P (domain_list s)\<rbrace> arch_get_sanitise_register_info t \<lbrace>\<lambda>_ s. P (domain_list s)\<rbrace>"
-  assumes arch_get_sanitise_register_info_domain_start_index_inv'[wp]:
-    "\<And>P t. arch_get_sanitise_register_info t \<lbrace>\<lambda>s::det_state. P (domain_start_index s)\<rbrace>"
-  assumes arch_switch_to_idle_thread_domain_list_inv'[wp]:
-    "\<And>P. \<lbrace>\<lambda>s::det_state. P (domain_list s)\<rbrace> arch_switch_to_idle_thread \<lbrace>\<lambda>_ s. P (domain_list s)\<rbrace>"
-  assumes arch_switch_to_idle_thread_domain_start_index_inv'[wp]:
-    "\<And>P. arch_switch_to_idle_thread \<lbrace>\<lambda>s::det_state. P (domain_start_index s)\<rbrace>"
-  assumes handle_arch_fault_reply_domain_list_inv'[wp]:
-    "\<And>P f t x y. \<lbrace>\<lambda>s::det_state. P (domain_list s)\<rbrace> handle_arch_fault_reply f t x y \<lbrace>\<lambda>_ s. P (domain_list s)\<rbrace>"
-  assumes handle_arch_fault_reply_domain_start_index_inv'[wp]:
-    "\<And>P f t x y. handle_arch_fault_reply f t x y \<lbrace>\<lambda>s::det_state. P (domain_start_index s)\<rbrace>"
-  assumes init_arch_objects_domain_list_inv'[wp]:
-    "\<And>P t d p n s r. \<lbrace>\<lambda>s::det_state. P (domain_list s)\<rbrace> init_arch_objects t d p n s r \<lbrace>\<lambda>_ s. P (domain_list s)\<rbrace>"
-  assumes init_arch_objects_domain_start_index_inv'[wp]:
-    "\<And>P t d p n s r. init_arch_objects t d p n s r \<lbrace>\<lambda>s::det_state. P (domain_start_index s)\<rbrace>"
-  assumes arch_post_modify_registers_domain_list_inv'[wp]:
-    "\<And>P t p. \<lbrace>\<lambda>s::det_state. P (domain_list s)\<rbrace> arch_post_modify_registers t p \<lbrace>\<lambda>_ s. P (domain_list s)\<rbrace>"
-  assumes arch_post_modify_registers_domain_start_index_inv'[wp]:
-    "\<And>P t p. arch_post_modify_registers t p \<lbrace>\<lambda>s::det_state. P (domain_start_index s)\<rbrace>"
-  assumes arch_invoke_irq_control_domain_list_inv'[wp]:
-    "\<And>P i. \<lbrace>\<lambda>s::det_state. P (domain_list s)\<rbrace> arch_invoke_irq_control i \<lbrace>\<lambda>_ s. P (domain_list s)\<rbrace>"
-  assumes arch_invoke_irq_control_domain_start_idnex_inv'[wp]:
-    "\<And>P i. arch_invoke_irq_control i \<lbrace>\<lambda>s::det_state. P (domain_start_index s)\<rbrace>"
-  assumes handle_vm_fault_domain_list_inv'[wp]:
-    "\<And>P t f. \<lbrace>\<lambda>s::det_state. P (domain_list s)\<rbrace> handle_vm_fault t f \<lbrace>\<lambda>_ s. P (domain_list s)\<rbrace>"
-  assumes handle_vm_fault_domain_start_index_inv'[wp]:
-    "\<And>P t f. handle_vm_fault t f \<lbrace>\<lambda>s::det_state. P (domain_start_index s)\<rbrace>"
-  assumes prepare_thread_delete_domain_list_inv'[wp]:
-    "\<And>P t. \<lbrace>\<lambda>s::det_state. P (domain_list s)\<rbrace> prepare_thread_delete t \<lbrace>\<lambda>_ s. P (domain_list s)\<rbrace>"
-  assumes prepare_thread_delete_domain_start_index_inv'[wp]:
-    "\<And>P t. prepare_thread_delete t \<lbrace>\<lambda>s::det_state. P (domain_start_index s)\<rbrace>"
-  assumes finalise_cap_domain_time_inv'[wp]:
-    "\<And>P cap fin. \<lbrace>\<lambda>s::det_state. P (domain_time s)\<rbrace> arch_finalise_cap cap fin \<lbrace>\<lambda>_ s. P (domain_time s)\<rbrace>"
-  assumes arch_activate_idle_thread_domain_time_inv'[wp]:
-    "\<And>P t. \<lbrace>\<lambda>s::det_state. P (domain_time s)\<rbrace> arch_activate_idle_thread t \<lbrace>\<lambda>_ s. P (domain_time s)\<rbrace>"
-  assumes arch_switch_to_thread_domain_time_inv'[wp]:
-    "\<And>P t. \<lbrace>\<lambda>s::det_state. P (domain_time s)\<rbrace> arch_switch_to_thread t \<lbrace>\<lambda>_ s. P (domain_time s)\<rbrace>"
-  assumes arch_get_sanitise_register_info_domain_time_inv'[wp]:
-    "\<And>P t. \<lbrace>\<lambda>s::det_state. P (domain_time s)\<rbrace> arch_get_sanitise_register_info t \<lbrace>\<lambda>_ s. P (domain_time s)\<rbrace>"
-  assumes arch_switch_to_idle_thread_domain_time_inv'[wp]:
-    "\<And>P. \<lbrace>\<lambda>s::det_state. P (domain_time s)\<rbrace> arch_switch_to_idle_thread \<lbrace>\<lambda>_ s. P (domain_time s)\<rbrace>"
-  assumes handle_arch_fault_reply_domain_time_inv'[wp]:
-    "\<And>P f t x y. \<lbrace>\<lambda>s::det_state. P (domain_time s)\<rbrace> handle_arch_fault_reply f t x y \<lbrace>\<lambda>_ s. P (domain_time s)\<rbrace>"
-  assumes init_arch_objects_domain_time_inv'[wp]:
-    "\<And>P t d p n s r. \<lbrace>\<lambda>s::det_state. P (domain_time s)\<rbrace> init_arch_objects t d p n s r \<lbrace>\<lambda>_ s. P (domain_time s)\<rbrace>"
-  assumes arch_post_modify_registers_domain_time_inv'[wp]:
-    "\<And>P t p. \<lbrace>\<lambda>s::det_state. P (domain_time s)\<rbrace> arch_post_modify_registers t p \<lbrace>\<lambda>_ s. P (domain_time s)\<rbrace>"
-  assumes arch_invoke_irq_control_domain_time_inv'[wp]:
-    "\<And>P i. \<lbrace>\<lambda>s::det_state. P (domain_time s)\<rbrace> arch_invoke_irq_control i \<lbrace>\<lambda>_ s. P (domain_time s)\<rbrace>"
-  assumes handle_vm_fault_domain_time_inv'[wp]:
-    "\<And>P t f. \<lbrace>\<lambda>s::det_state. P (domain_time s)\<rbrace> handle_vm_fault t f \<lbrace>\<lambda>_ s. P (domain_time s)\<rbrace>"
-  assumes prepare_thread_delete_domain_time_inv'[wp]:
-    "\<And>P t. \<lbrace>\<lambda>s::det_state. P (domain_time s)\<rbrace> prepare_thread_delete t \<lbrace>\<lambda>_ s. P (domain_time s)\<rbrace>"
-  assumes arch_post_cap_deletion_domain_time_inv'[wp]:
-    "\<And>P ft. \<lbrace>\<lambda>s::det_state. P (domain_time s)\<rbrace> arch_post_cap_deletion ft \<lbrace>\<lambda>_ s. P (domain_time s)\<rbrace>"
-  assumes arch_post_cap_deletion_domain_list_inv'[wp]:
-    "\<And>P ft. \<lbrace>\<lambda>s::det_state. P (domain_list s)\<rbrace> arch_post_cap_deletion ft \<lbrace>\<lambda>_ s. P (domain_list s)\<rbrace>"
-  assumes arch_post_cap_deletion_domain_start_index_inv'[wp]:
-    "\<And>P ft. arch_post_cap_deletion ft \<lbrace>\<lambda>s::det_state. P (domain_start_index s)\<rbrace>"
-  assumes arch_invoke_irq_handler_domain_list_inv'[wp]:
-    "\<And>P i. arch_invoke_irq_handler i \<lbrace>\<lambda>s::det_state. P (domain_list s)\<rbrace>"
-  assumes arch_invoke_irq_handler_domain_start_index_inv'[wp]:
-    "\<And>P i. arch_invoke_irq_handler i \<lbrace>\<lambda>s::det_state. P (domain_start_index s)\<rbrace>"
-  assumes arch_invoke_irq_handler_domain_time_inv'[wp]:
-    "\<And>P i. arch_invoke_irq_handler i \<lbrace>\<lambda>s::det_state. P (domain_time s)\<rbrace>"
-  assumes arch_prepare_next_domain_domain_list_inv'[wp]:
-    "\<And>P. arch_prepare_next_domain \<lbrace>\<lambda>s::det_state. P (domain_list s)\<rbrace>"
-  assumes arch_prepare_next_domain_domain_start_index_inv'[wp]:
-    "\<And>P. arch_prepare_next_domain \<lbrace>\<lambda>s::det_state. P (domain_start_index s)\<rbrace>"
-  assumes arch_prepare_set_domain_domain_list_inv'[wp]:
-    "\<And>P t d. arch_prepare_set_domain t d \<lbrace>\<lambda>s::det_state. P (domain_list s)\<rbrace>"
-  assumes arch_prepare_set_domain_domain_start_index_inv'[wp]:
-    "\<And>P t d. arch_prepare_set_domain t d \<lbrace>\<lambda>s::det_state. P (domain_start_index s)\<rbrace>"
-  assumes arch_post_set_flags_domain_list_inv'[wp]:
-    "\<And>P t fs. arch_post_set_flags t fs \<lbrace>\<lambda>s::det_state. P (domain_list s)\<rbrace>"
-  assumes arch_post_set_flags_domain_start_index_inv'[wp]:
-    "\<And>P t fs. arch_post_set_flags t fs \<lbrace>\<lambda>s::det_state. P (domain_start_index s)\<rbrace>"
-  assumes arch_prepare_set_domain_domain_time_inv'[wp]:
-    "\<And>P t d. arch_prepare_set_domain t d \<lbrace>\<lambda>s::det_state. P (domain_time s)\<rbrace>"
-  assumes arch_post_set_flags_domain_time_inv'[wp]:
-    "\<And>P t fs. arch_post_set_flags t fs \<lbrace>\<lambda>s::det_state. P (domain_time s)\<rbrace>"
+  assumes finalise_cap_domain_fields_inv[wp]:
+    "\<And>P cap fin. arch_finalise_cap cap fin \<lbrace>domain_fields P\<rbrace>"
+  assumes arch_activate_idle_thread_domain_fields_inv[wp]:
+    "\<And>P t. arch_activate_idle_thread t \<lbrace>domain_fields P\<rbrace>"
+  assumes arch_switch_to_thread_domain_fields_inv[wp]:
+    "\<And>P t. arch_switch_to_thread t \<lbrace>domain_fields P\<rbrace>"
+  assumes arch_get_sanitise_register_info_domain_fields_inv[wp]:
+    "\<And>P t. arch_get_sanitise_register_info t \<lbrace>domain_fields P\<rbrace>"
+  assumes arch_switch_to_idle_thread_domain_fields_inv[wp]:
+    "\<And>P. arch_switch_to_idle_thread \<lbrace>domain_fields P\<rbrace>"
+  assumes handle_arch_fault_reply_domain_fields_inv[wp]:
+    "\<And>P f t x y. handle_arch_fault_reply f t x y \<lbrace>domain_fields P\<rbrace>"
+  assumes init_arch_objects_domain_fields_inv[wp]:
+    "\<And>P t d p n s r. init_arch_objects t d p n s r \<lbrace>domain_fields P\<rbrace>"
+  assumes arch_post_modify_registers_domain_fields_inv[wp]:
+    "\<And>P t p. arch_post_modify_registers t p \<lbrace>domain_fields P\<rbrace>"
+  assumes arch_invoke_irq_control_domain_fields_inv[wp]:
+    "\<And>P i. arch_invoke_irq_control i \<lbrace>domain_fields P\<rbrace>"
+  assumes handle_vm_fault_domain_fields_inv[wp]:
+    "\<And>P t f. handle_vm_fault t f \<lbrace>domain_fields P\<rbrace>"
+  assumes prepare_thread_delete_domain_fields_inv[wp]:
+    "\<And>P t. prepare_thread_delete t \<lbrace>domain_fields P\<rbrace>"
+  assumes arch_post_cap_deletion_domain_fields_inv[wp]:
+    "\<And>P ft. arch_post_cap_deletion ft \<lbrace>domain_fields P\<rbrace>"
+  assumes arch_invoke_irq_handler_domain_fields_inv[wp]:
+    "\<And>P i. arch_invoke_irq_handler i \<lbrace>domain_fields P\<rbrace>"
+  assumes arch_prepare_next_domain_domain_fields_inv[wp]:
+    "\<And>P. arch_prepare_next_domain \<lbrace>domain_fields P\<rbrace>"
+  assumes arch_prepare_set_domain_domain_fields_inv[wp]:
+    "\<And>P t d. arch_prepare_set_domain t d \<lbrace>domain_fields P\<rbrace>"
+  assumes arch_post_set_flags_domain_fields_inv[wp]:
+    "\<And>P t fs. arch_post_set_flags t fs \<lbrace>domain_fields P\<rbrace>"
 
 crunch update_restart_pc
-  for domain_list[wp]: "\<lambda>s. P (domain_list s)"
-  and domain_time[wp]: "\<lambda>s. P (domain_time s)"
-  and domain_start_index[wp]: "\<lambda>s. P (domain_start_index s)"
+  for domain_fields[wp]: "domain_fields P"
   (wp: crunch_wps)
 
 locale DetSchedDomainTime_AI_2 = DetSchedDomainTime_AI +
-  assumes handle_hypervisor_fault_domain_list_inv'[wp]:
-    "\<And>P t f. \<lbrace>\<lambda>s. P (domain_list s)\<rbrace> handle_hypervisor_fault t f \<lbrace>\<lambda>_ s::det_state. P (domain_list s)\<rbrace>"
-  assumes handle_hypervisor_fault_domain_start_index_inv'[wp]:
-    "\<And>P t f. handle_hypervisor_fault t f \<lbrace>\<lambda>s::det_state. P (domain_start_index s)\<rbrace>"
-  assumes handle_hypervisor_fault_domain_time_inv'[wp]:
-    "\<And>P t f. \<lbrace>\<lambda>s. P (domain_time s)\<rbrace> handle_hypervisor_fault t f \<lbrace>\<lambda>_ s::det_state. P (domain_time s)\<rbrace>"
-  assumes arch_perform_invocation_domain_list_inv'[wp]:
-    "\<And>P i. \<lbrace>\<lambda>s. P (domain_list s)\<rbrace> arch_perform_invocation i \<lbrace>\<lambda>_ s::det_state. P (domain_list s)\<rbrace>"
-  assumes arch_perform_invocation_domain_start_index_inv'[wp]:
-    "\<And>P i. arch_perform_invocation i \<lbrace>\<lambda>s::det_state. P (domain_start_index s)\<rbrace>"
-  assumes arch_perform_invocation_domain_time_inv'[wp]:
-    "\<And>P i. \<lbrace>\<lambda>s. P (domain_time s)\<rbrace> arch_perform_invocation i \<lbrace>\<lambda>_ s::det_state. P (domain_time s)\<rbrace>"
+  assumes handle_hypervisor_fault_domain_fields_invs[wp]:
+    "\<And>P t f. handle_hypervisor_fault t f \<lbrace>domain_fields P\<rbrace>"
+  assumes arch_perform_invocation_domain_fields_invs[wp]:
+    "\<And>P i. arch_perform_invocation i \<lbrace>domain_fields P\<rbrace>"
   assumes handle_interrupt_valid_domain_time:
     "\<And>i.
       \<lbrace>\<lambda>s :: det_ext state. 0 < domain_time s \<rbrace>
         handle_interrupt i
       \<lbrace>\<lambda>rv s.  domain_time s = 0 \<longrightarrow> scheduler_action s = choose_new_thread \<rbrace>"
-  assumes handle_reserved_irq_some_time_inv'[wp]:
-    "\<And>P irq. \<lbrace>\<lambda>s. P (domain_time s)\<rbrace> handle_reserved_irq irq \<lbrace>\<lambda>_ s::det_state. P (domain_time s)\<rbrace>"
-  assumes handle_reserved_irq_domain_list_inv'[wp]:
-    "\<And>P irq. \<lbrace>\<lambda>s. P (domain_list s)\<rbrace> handle_reserved_irq irq \<lbrace>\<lambda>_ s::det_state. P (domain_list s)\<rbrace>"
-  assumes handle_reserved_irq_domain_start_index_inv'[wp]:
-    "\<And>P irq. handle_reserved_irq irq \<lbrace>\<lambda>s::det_state. P (domain_start_index s)\<rbrace>"
-  assumes arch_mask_irq_signal_domain_list_inv'[wp]:
-    "\<And>P irq. arch_mask_irq_signal irq \<lbrace>\<lambda>s::det_state. P (domain_list s)\<rbrace>"
-  assumes arch_mask_irq_signal_domain_start_index_inv'[wp]:
-    "\<And>P irq. arch_mask_irq_signal irq \<lbrace>\<lambda>s::det_state. P (domain_start_index s)\<rbrace>"
-  assumes arch_mask_irq_signal_domain_time_inv'[wp]:
-    "\<And>P irq. arch_mask_irq_signal irq \<lbrace>\<lambda>s::det_state. P (domain_time s)\<rbrace>"
-  assumes handle_spurious_irq_domain_time_inv'[wp]:
-    "\<And>P. handle_spurious_irq \<lbrace>\<lambda>s::det_state. P (domain_time s)\<rbrace>"
-  assumes handle_spurious_irq_domain_list_inv'[wp]:
-    "\<And>P. handle_spurious_irq \<lbrace>\<lambda>s::det_state. P (domain_list s)\<rbrace>"
-  assumes handle_spurious_irq_domain_start_index_inv'[wp]:
-    "\<And>P. handle_spurious_irq \<lbrace>\<lambda>s::det_state. P (domain_start_index s)\<rbrace>"
+  assumes handle_reserved_irq_domain_fields_invs[wp]:
+    "\<And>P irq. handle_reserved_irq irq \<lbrace>domain_fields P\<rbrace>"
+  assumes arch_mask_irq_signal_domain_fields_invs[wp]:
+    "\<And>P irq. arch_mask_irq_signal irq \<lbrace>domain_fields P\<rbrace>"
+  assumes handle_spurious_irq_domain_fields_invs[wp]:
+    "\<And>P. handle_spurious_irq \<lbrace>domain_fields P\<rbrace>"
   assumes handle_spurious_irq_scheduler_action[wp]:
-    "handle_spurious_irq \<lbrace>\<lambda>s::det_state. P (scheduler_action s) \<rbrace>"
+    "\<And>P. handle_spurious_irq \<lbrace>\<lambda>s::det_state. P (scheduler_action s)\<rbrace>"
 
 context DetSchedDomainTime_AI begin
 
 crunch
   cap_swap_for_delete, empty_slot, get_object, get_cap, tcb_sched_action
-  for domain_list_inv[wp]: "\<lambda>s::det_state. P (domain_list s)"
-  and domain_start_index_inv[wp]: "\<lambda>s::det_state. P (domain_start_index s)"
+  for domain_fields_invs[wp]: "domain_fields P"
 
 crunch finalise_cap
-  for domain_list_inv[wp]: "\<lambda>s::det_state. P (domain_list s)"
-  and domain_start_index_inv[wp]: "\<lambda>s::det_state. P (domain_start_index s)"
+  for domain_fields_invs[wp]: "domain_fields P"
   (wp: crunch_wps unless_wp select_inv simp: crunch_simps)
 
-lemma rec_del_domain_list[wp]:
-  "rec_del call \<lbrace>\<lambda>s::det_state. P (domain_list s)\<rbrace>"
-  by (wp rec_del_preservation preemption_point_inv' | simp)+
-
-lemma rec_del_domain_start_index[wp]:
-  "rec_del call \<lbrace>\<lambda>s::det_state. P (domain_start_index s)\<rbrace>"
+lemma rec_del_domain_fields_invst[wp]:
+  "rec_del call \<lbrace>domain_fields P\<rbrace>"
   by (wp rec_del_preservation preemption_point_inv' | simp)+
 
 crunch cap_delete, activate_thread
-  for domain_list_inv[wp]: "\<lambda>s::det_state. P (domain_list s)"
-  and domain_start_index_inv[wp]: "\<lambda>s::det_state. P (domain_start_index s)"
+  for domain_fields_invs[wp]: "domain_fields P"
 
 crunch schedule
-  for domain_list_inv[wp]: "\<lambda>s::det_state. P (domain_list s)"
+  for domain_list_invs[wp]: "\<lambda>s::det_state. P (domain_list s)"
   and domain_start_index_inv[wp]: "\<lambda>s::det_state. P (domain_start_index s)"
   (wp: hoare_drop_imp dxo_wp_weak simp: Let_def)
 
 end
 
 crunch (in DetSchedDomainTime_AI_2) handle_interrupt
-  for domain_list_inv[wp]: "\<lambda>s::det_state. P (domain_list s)"
-  and domain_start_index_inv[wp]: "\<lambda>s::det_state. P (domain_start_index s)"
+  for dlist_fields_inv[wp]: "dlist_fields P"
 
-crunch cap_insert
- for domain_list_inv[wp]: "\<lambda>s::det_state. P (domain_list s)"
-  and domain_start_index_inv[wp]: "\<lambda>s::det_state. P (domain_start_index s)"
-  (wp: hoare_drop_imps)
-
-crunch
-  lookup_cap_and_slot, set_extra_badge
-  for domain_list_inv[wp]: "\<lambda>s. P (domain_list s)"
-  and domain_start_index_inv[wp]: "\<lambda>s::det_state. P (domain_start_index s)"
+crunch cap_insert, lookup_cap_and_slot, set_extra_badge
+  for domain_fields_invs[wp]: "domain_fields P"
   (wp: hoare_drop_imps)
 
 context DetSchedDomainTime_AI begin
+
 crunch do_ipc_transfer
-  for domain_list_inv[wp]: "\<lambda>s::det_state. P (domain_list s)"
-  and domain_start_index_inv[wp]: "\<lambda>s::det_state. P (domain_start_index s)"
+  for domain_fields_invs[wp]: "domain_fields P"
   (wp: crunch_wps simp: zipWithM_x_mapM rule: transfer_caps_loop_pres)
 
 crunch handle_fault
-  for domain_list_inv[wp]: "\<lambda>s::det_state. P (domain_list s)"
-  and domain_start_index_inv[wp]: "\<lambda>s::det_state. P (domain_start_index s)"
+  for domain_fields_invs[wp]: "domain_fields P"
   (wp: mapM_wp hoare_drop_imps simp: crunch_simps ignore:copy_mrs)
-
 
 crunch
   reply_from_kernel, create_cap, retype_region, do_reply_transfer
-  for domain_list_inv[wp]: "\<lambda>s::det_state. P (domain_list s)"
-  and domain_start_index_inv[wp]: "\<lambda>s::det_state. P (domain_start_index s)"
+  for domain_fields_invs[wp]: "domain_fields P"
   (wp: hoare_drop_imps)
+
 end
 
 crunch delete_objects
-  for domain_list_inv[wp]: "\<lambda>s :: det_ext state. P (domain_list s)"
-  and domain_start_index_inv[wp]: "\<lambda>s::det_state. P (domain_start_index s)"
+  for domain_fields_invs[wp]: "domain_fields P"
   (wp: crunch_wps simp: detype_def)
 
 crunch preemption_point
-  for domain_list_inv[wp]: "\<lambda>s::det_state. P (domain_list s)"
-  and domain_start_index_inv[wp]: "\<lambda>s::det_state. P (domain_start_index s)"
+  for domain_fields_invs[wp]: "domain_fields P"
   (wp: OR_choiceE_weak_wp ignore_del: preemption_point)
 
 crunch reset_untyped_cap
-  for domain_list_inv[wp]: "\<lambda>s::det_state. P (domain_list s)"
-  and domain_start_index_inv[wp]: "\<lambda>s::det_state. P (domain_start_index s)"
+  for domain_fields_invs[wp]: "domain_fields P"
   (wp: crunch_wps unless_wp mapME_x_inv_wp select_inv
    simp: crunch_simps)
 
 context DetSchedDomainTime_AI begin
 
 crunch invoke_untyped
-  for domain_list_inv[wp]: "\<lambda>s::det_state. P (domain_list s)"
-  and domain_start_index_inv[wp]: "\<lambda>s::det_state. P (domain_start_index s)"
+  for domain_fields_invs[wp]: "domain_fields P"
   (wp: crunch_wps
-    simp: crunch_simps mapM_x_defsym)
+   simp: crunch_simps mapM_x_defsym)
 
 crunch
   invoke_tcb, invoke_set_domain, invoke_irq_control, invoke_irq_handler
-  for domain_list_inv[wp]: "\<lambda>s::det_state. P (domain_list s)"
-  and domain_start_index_inv[wp]: "\<lambda>s::det_state. P (domain_start_index s)"
+  for domain_fields_invs[wp]: "domain_fields P"
   (wp: crunch_wps check_cap_inv)
 
 end
 
 crunch cap_move
-  for domain_list_inv[wp]: "\<lambda>s::det_state. P (domain_list s)"
-  and domain_start_index_inv[wp]: "\<lambda>s::det_state. P (domain_start_index s)"
+  for domain_fields_invs[wp]: "domain_fields P"
 
 context DetSchedDomainTime_AI begin
 
-lemma cap_revoke_domain_list_inv[wp]:
-  "cap_revoke a \<lbrace>\<lambda>s::det_ext state. P (domain_list s)\<rbrace>"
-  by (rule cap_revoke_preservation2)
-     (wp preemption_point_inv'|simp)+
-
-lemma cap_revoke_domain_start_index_inv[wp]:
-  "cap_revoke a \<lbrace>\<lambda>s::det_ext state. P (domain_start_index s)\<rbrace>"
+lemma cap_revoke_domain_fields_invs[wp]:
+  "cap_revoke a \<lbrace>domain_fields P\<rbrace>"
   by (rule cap_revoke_preservation2)
      (wp preemption_point_inv'|simp)+
 
 end
 
 crunch cancel_badged_sends
-  for domain_list_inv[wp]: "\<lambda>s. P (domain_list s)"
-  and domain_start_index_inv[wp]: "\<lambda>s::det_state. P (domain_start_index s)"
+  for domain_fields_invs[wp]: "domain_fields P"
   (ignore: filterM clearMemory
      simp: filterM_mapM crunch_simps
        wp: crunch_wps)
@@ -310,23 +218,18 @@ lemma handle_spurious_irq_valid_domain[wp]:
   "handle_spurious_irq \<lbrace>\<lambda>s::det_state. domain_time s = 0 \<longrightarrow> scheduler_action s = choose_new_thread \<rbrace>"
   by (wp | wps)+
 
-lemma invoke_cnode_domain_list_inv[wp]:
-  "invoke_cnode i \<lbrace>\<lambda>s :: det_ext state. P (domain_list s) \<rbrace>"
+lemma invoke_cnode_fields_invs[wp]:
+  "invoke_cnode i \<lbrace>domain_fields P\<rbrace>"
   by (wpsimp wp: crunch_wps cap_move_src_slot_Null hoare_drop_imps hoare_vcg_all_lift
              simp: invoke_cnode_def crunch_simps
              split_del: if_split)
 
-lemma invoke_cnode_domain_start_index_inv[wp]:
-  "invoke_cnode i \<lbrace>\<lambda>s :: det_ext state. P (domain_start_index s) \<rbrace>"
-  by (wpsimp wp: crunch_wps cap_move_src_slot_Null hoare_drop_imps hoare_vcg_all_lift
-             simp: invoke_cnode_def crunch_simps
-             split_del: if_split)
+crunch handle_recv, handle_yield, handle_reply, handle_vm_fault
+  for dlist_fields_invs[wp]: "domain_fields P"
+  (wp: crunch_wps simp: crunch_simps)
 
-crunch
-  handle_recv, handle_yield, handle_reply, handle_vm_fault, handle_hypervisor_fault,
-  maybe_handle_interrupt
-  for domain_list_inv[wp]: "\<lambda>s::det_state. P (domain_list s)"
-  and domain_start_index_inv[wp]: "\<lambda>s::det_state. P (domain_start_index s)"
+crunch maybe_handle_interrupt
+  for dlist_fields_invs[wp]: "dlist_fields P"
   (wp: crunch_wps simp: crunch_simps)
 
 lemma domain_set_start_valid_domain_list_inv[wp]:
@@ -335,7 +238,7 @@ lemma domain_set_start_valid_domain_list_inv[wp]:
    \<lbrace>\<lambda>_ s::det_state. valid_domain_list s\<rbrace>"
   unfolding domain_set_start_def
   apply (wpsimp wp: valid_domain_list_lift[of reschedule_required])
-  apply (simp add: valid_domain_inv_def valid_domain_list_def domain_end_marker_def)
+  apply (fastforce simp add: valid_domain_inv_def valid_domain_list_def domain_end_marker_def)
   done
 
 lemma domain_schedule_configure_valid_domain_list_inv[wp]:
@@ -392,12 +295,25 @@ lemma handle_event_domain_list_inv[wp]:
    \<lbrace>\<lambda>_ s::det_state. valid_domain_list s\<rbrace>"
   by (cases e; (wpsimp | wp valid_domain_list_lift)+)
 
+lemma next_domain_valid_domain_list[wp]:
+  "next_domain \<lbrace>\<lambda>s::det_state. valid_domain_list s\<rbrace>"
+  unfolding next_domain_def
+  apply (wpsimp wp: dxo_wp_weak)
+  apply (clarsimp simp: valid_domain_list_def Let_def domain_end_marker_def)
+  using less_Suc_eq
+  apply fastforce
+  done
+
+crunch schedule
+  for valid_domain_list[wp]: "\<lambda>s::det_state. valid_domain_list s"
+  (wp: crunch_wps)
+
 lemma call_kernel_domain_list_inv_det_ext:
   "\<lbrace>valid_domain_list and invs\<rbrace>
      (call_kernel e) :: (unit,det_ext) s_monad
    \<lbrace>\<lambda>_. valid_domain_list\<rbrace>"
   unfolding call_kernel_def
-  by (wpsimp | wp valid_domain_list_lift)+
+  by wpsimp
 
 end
 
@@ -424,87 +340,18 @@ crunch send_signal
   for domain_time_inv[wp]: "\<lambda>s::det_state. P (domain_time s)"
   (wp: hoare_drop_imps mapM_x_wp_inv simp: crunch_simps unless_def)
 
-crunch
-  cap_swap_for_delete, empty_slot, get_object, get_cap, tcb_sched_action
-  for domain_time_inv[wp]: "\<lambda>s::det_state. P (domain_time s)"
-
-crunch finalise_cap
-  for domain_time_inv[wp]: "\<lambda>s::det_state. P (domain_time s)"
-  (wp: crunch_wps hoare_drop_imps unless_wp select_inv mapM_wp
-       subset_refl if_fun_split simp: crunch_simps ignore: tcb_sched_action)
-
-lemma rec_del_domain_time[wp]:
-  "\<lbrace>\<lambda>s. P (domain_time s)\<rbrace> rec_del call \<lbrace>\<lambda>rv s::det_state. P (domain_time s)\<rbrace>"
-  by (wp rec_del_preservation preemption_point_inv' | simp)+
-
-crunch
-  cap_delete, activate_thread, lookup_cap_and_slot
-  for domain_time_inv[wp]: "\<lambda>s::det_state. P (domain_time s)"
-
 end
-
-crunch cap_insert
-  for domain_time_inv[wp]: "\<lambda>s::det_state. P (domain_time s)"
-  (wp: hoare_drop_imps)
 
 crunch set_extra_badge
   for domain_time_inv[wp]: "\<lambda>s. P (domain_time s)"
 
 context DetSchedDomainTime_AI begin
 
-crunch do_ipc_transfer
-  for domain_time_inv[wp]: "\<lambda>s::det_state. P (domain_time s)"
-  (wp: crunch_wps simp: zipWithM_x_mapM rule: transfer_caps_loop_pres)
-
-crunch handle_fault
-  for domain_time_inv[wp]: "\<lambda>s::det_state. P (domain_time s)"
-  (wp: mapM_wp hoare_drop_imps simp: crunch_simps ignore:copy_mrs)
-
-crunch
-  reply_from_kernel, create_cap, retype_region
-  for domain_time_inv[wp]: "\<lambda>s::det_state. P (domain_time s)"
-
-crunch do_reply_transfer
-  for domain_time_inv[wp]: "\<lambda>s::det_state. P (domain_time s)"
-  (wp: hoare_drop_imps)
-end
-
-crunch delete_objects
-  for domain_time_inv[wp]: "\<lambda>s :: det_ext state. P (domain_time s)"
-  (wp: crunch_wps simp: detype_def)
-
-crunch preemption_point
-  for domain_time_inv[wp]: "\<lambda>s::det_state. P (domain_time s)"
-  (wp: OR_choiceE_weak_wp ignore_del: preemption_point)
-
-crunch reset_untyped_cap
-  for domain_time_inv[wp]: "\<lambda>s::det_state. P (domain_time s)"
-  (wp: crunch_wps unless_wp mapME_x_inv_wp select_inv
-   simp: crunch_simps)
-
-context DetSchedDomainTime_AI begin
-
-crunch invoke_untyped
-  for domain_time_inv[wp]: "\<lambda>s::det_state. P (domain_time s)"
-  (wp: crunch_wps
-    simp: crunch_simps mapM_x_defsym)
-
 crunch
   invoke_tcb, invoke_set_domain, domain_schedule_configure, invoke_irq_control, invoke_irq_handler
   for domain_time_inv[wp]: "\<lambda>s::det_state. P (domain_time s)"
   (wp: crunch_wps check_cap_inv)
 
-end
-
-crunch cap_move
-  for domain_time_inv[wp]: "\<lambda>s::det_state. P (domain_time s)"
-
-context DetSchedDomainTime_AI begin
-lemma cap_revoke_domain_time_inv[wp]:
-  "\<lbrace>(\<lambda>s :: det_ext state. P (domain_time s))\<rbrace> cap_revoke a \<lbrace>\<lambda>rv s. P (domain_time s)\<rbrace>"
-  apply (rule cap_revoke_preservation2)
-  apply (wp preemption_point_inv'|simp)+
-  done
 end
 
 crunch cancel_badged_sends
@@ -534,20 +381,6 @@ lemma domain_set_start_valid_domain_time[wp]:
   by (wpsimp wp: reschedule_required_valid_domain_time)
 
 context DetSchedDomainTime_AI_2 begin
-
-lemma invoke_cnode_domain_time_inv[wp]:
-  "\<lbrace>\<lambda>s :: det_ext state. P (domain_time s)\<rbrace>
-     invoke_cnode i
-   \<lbrace>\<lambda>rv s. P (domain_time s) \<rbrace>"
-  apply (rule hoare_pre)
-   apply (wp crunch_wps cap_move_src_slot_Null hoare_drop_imps hoare_vcg_all_lift
-          | wpc | simp add: invoke_cnode_def crunch_simps split del: if_split)+
-  done
-
-crunch
-  handle_recv, handle_yield, handle_reply, handle_vm_fault, handle_hypervisor_fault
-  for domain_time_inv[wp]: "\<lambda>s::det_state. P (domain_time s)"
-  (wp: crunch_wps simp: crunch_simps)
 
 lemma domain_time_strg:
   "0 < domain_time s \<Longrightarrow> domain_time s = 0 \<longrightarrow> scheduler_action s = choose_new_thread"
@@ -642,8 +475,12 @@ lemma next_domain_domain_time_left[wp]:
   "\<lbrace> valid_domain_list \<rbrace> next_domain \<lbrace>\<lambda>_ s. 0 < domain_time s \<rbrace>"
   unfolding next_domain_def Let_def
   apply (wpsimp wp: dxo_wp_weak)
-  apply (fastforce simp: valid_domain_list_def all_set_conv_all_nth word_greater_zero_iff
+  apply (clarsimp simp: valid_domain_list_def all_set_conv_all_nth word_greater_zero_iff
                          ucast_eq_0 is_up domain_end_marker_def not_le)
+  apply (rule conjI)
+   apply fastforce
+  apply (metis (mono_tags, lifting) less_imp_diff_less linorder_neqE_nat not_less_eq prod.simps(2)
+                                    surjective_pairing)
   done
 
 context DetSchedDomainTime_AI begin
