proof/invariant-abstract/ARM_HYP/ArchDetSchedDomainTime_AI.thy
@@ -16,63 +16,38 @@ crunch
   vcpu_update, vcpu_save_reg, vgic_update, vcpu_enable, vcpu_disable, vcpu_restore,
   vcpu_write_reg, vcpu_read_reg, vcpu_save, vcpu_switch, set_vcpu, vgic_update_lr,
   read_vcpu_register, write_vcpu_register
-  for domain_list_inv[wp]: "\<lambda>s. P (domain_list s)"
-  and domain_time_inv[wp]: "\<lambda>s. P (domain_time s)"
-  and domain_start_index_inv[wp, DetSchedDomainTime_AI_assms]: "\<lambda>s::det_state. P (domain_start_index s)"
+  for domain_fields_invs[wp, DetSchedDomainTime_AI_assms]: "domain_fields P"
   (wp: crunch_wps simp: crunch_simps)
-
-crunch arch_finalise_cap
-  for domain_list_inv[wp, DetSchedDomainTime_AI_assms]: "\<lambda>s. P (domain_list s)"
-  and domain_start_index_inv[wp, DetSchedDomainTime_AI_assms]: "\<lambda>s::det_state. P (domain_start_index s)"
-  (wp: hoare_drop_imps mapM_wp subset_refl simp: crunch_simps)
 
 crunch
   arch_activate_idle_thread, arch_switch_to_thread, arch_switch_to_idle_thread,
-  handle_arch_fault_reply,
+  handle_arch_fault_reply, arch_finalise_cap,
   arch_invoke_irq_control, arch_get_sanitise_register_info,
   prepare_thread_delete, handle_hypervisor_fault, init_arch_objects,
   arch_post_modify_registers, arch_post_cap_deletion, handle_vm_fault,
-  arch_invoke_irq_handler, arch_prepare_next_domain, arch_prepare_set_domain, arch_post_set_flags
-  for domain_list_inv[wp, DetSchedDomainTime_AI_assms]: "\<lambda>s::det_state. P (domain_list s)"
-  and domain_start_index_inv[wp, DetSchedDomainTime_AI_assms]: "\<lambda>s::det_state. P (domain_start_index s)"
+  arch_invoke_irq_handler, arch_prepare_next_domain, arch_prepare_set_domain,
+  arch_post_set_flags, handle_spurious_irq, handle_reserved_irq,
+  arch_mask_irq_signal
+  for domain_fields_invs[wp, DetSchedDomainTime_AI_assms]: "domain_fields P"
   (simp: crunch_simps wp: mapM_wp' transfer_caps_loop_pres crunch_wps)
+
 declare init_arch_objects_exst[DetSchedDomainTime_AI_assms]
-
-crunch arch_finalise_cap, arch_get_sanitise_register_info
-  for domain_time_inv[wp, DetSchedDomainTime_AI_assms]: "\<lambda>s. P (domain_time s)"
-  (wp: hoare_drop_imps mapM_wp subset_refl simp: crunch_simps)
-
-crunch
-  arch_activate_idle_thread, arch_switch_to_thread, arch_switch_to_idle_thread,
-  handle_arch_fault_reply, init_arch_objects,
-  arch_invoke_irq_control, arch_get_sanitise_register_info,
-  prepare_thread_delete, handle_hypervisor_fault, handle_vm_fault,
-  arch_post_modify_registers, arch_post_cap_deletion,
-  arch_invoke_irq_handler, handle_reserved_irq, arch_mask_irq_signal,
-  arch_prepare_next_domain, arch_prepare_set_domain, arch_post_set_flags,
-  handle_spurious_irq
-  for domain_time_inv[wp, DetSchedDomainTime_AI_assms]: "\<lambda>s::det_state. P (domain_time s)"
-  and domain_start_index_inv[wp, DetSchedDomainTime_AI_assms]: "\<lambda>s::det_state. P (domain_start_index s)"
-  (simp: crunch_simps wp: transfer_caps_loop_pres crunch_wps)
 
 crunch handle_spurious_irq
   for scheduler_action[wp, DetSchedDomainTime_AI_assms]: "\<lambda>s. P (scheduler_action s)"
-  and domain_list_inv[wp, DetSchedDomainTime_AI_assms]: "\<lambda>s::det_state. P (domain_list s)"
 
 end
 
 global_interpretation DetSchedDomainTime_AI?: DetSchedDomainTime_AI
-  proof goal_cases
+proof goal_cases
   interpret Arch .
   case 1 show ?case by (unfold_locales; (fact DetSchedDomainTime_AI_assms)?)
-  qed
+qed
 
 context Arch begin arch_global_naming
 
 crunch arch_perform_invocation
-  for domain_time_inv[wp, DetSchedDomainTime_AI_assms]: "\<lambda>s::det_state. P (domain_time s)"
-  and domain_list_inv[wp, DetSchedDomainTime_AI_assms]: "\<lambda>s::det_state. P (domain_list s)"
-  and domain_start_index_inv[wp, DetSchedDomainTime_AI_assms]: "\<lambda>s::det_state. P (domain_start_index s)"
+  for domain_fields_invs[wp, DetSchedDomainTime_AI_assms]: "domain_fields P"
   (wp: crunch_wps check_cap_inv)
 
 lemma vgic_maintenance_valid_domain_time:
@@ -80,7 +55,7 @@ lemma vgic_maintenance_valid_domain_time:
     vgic_maintenance \<lbrace>\<lambda>y s. domain_time s = 0 \<longrightarrow> scheduler_action s = choose_new_thread\<rbrace>"
   unfolding vgic_maintenance_def
   apply (rule hoare_strengthen_post[where Q'="\<lambda>_ s. 0 < domain_time s"])
-   apply (wpsimp wp: handle_fault_domain_time_inv hoare_drop_imps)
+   apply (wpsimp wp: hoare_drop_imps)
   apply clarsimp
   done
 
@@ -89,7 +64,7 @@ lemma vppi_event_valid_domain_time:
     vppi_event irq \<lbrace>\<lambda>y s. domain_time s = 0 \<longrightarrow> scheduler_action s = choose_new_thread\<rbrace>"
   unfolding vppi_event_def
   apply (rule hoare_strengthen_post[where Q'="\<lambda>_ s. 0 < domain_time s"])
-   apply (wpsimp wp: handle_fault_domain_time_inv hoare_drop_imps)
+   apply (wpsimp wp: hoare_drop_imps)
   apply clarsimp
   done
 
@@ -142,16 +117,12 @@ lemma handle_interrupt_valid_domain_time [DetSchedDomainTime_AI_assms]:
    apply wpsimp+
   done
 
-crunch handle_reserved_irq, arch_mask_irq_signal
-  for domain_list_inv [wp, DetSchedDomainTime_AI_assms]: "\<lambda>s::det_state. P (domain_list s)"
-  (wp: crunch_wps mapM_wp subset_refl simp: crunch_simps)
-
 end
 
 global_interpretation DetSchedDomainTime_AI_2?: DetSchedDomainTime_AI_2
-  proof goal_cases
+proof goal_cases
   interpret Arch .
   case 1 show ?case by (unfold_locales; (fact DetSchedDomainTime_AI_assms)?)
-  qed
+qed
 
 end
