proof/invariant-abstract/RISCV64/ArchDetSchedDomainTime_AI.thy
@@ -12,34 +12,14 @@ context Arch begin arch_global_naming
 
 named_theorems DetSchedDomainTime_AI_assms
 
-crunch arch_finalise_cap
-  for domain_list_inv[wp, DetSchedDomainTime_AI_assms]: "\<lambda>s. P (domain_list s)"
-  (wp: hoare_drop_imps mapM_wp subset_refl simp: crunch_simps)
-
 crunch
   arch_activate_idle_thread, arch_switch_to_thread, arch_switch_to_idle_thread,
-  handle_arch_fault_reply,
+  handle_arch_fault_reply, arch_finalise_cap,
   arch_invoke_irq_control, arch_get_sanitise_register_info,
   prepare_thread_delete, handle_hypervisor_fault, init_arch_objects,
   arch_post_modify_registers, arch_post_cap_deletion, handle_vm_fault,
   arch_invoke_irq_handler, arch_prepare_next_domain, arch_prepare_set_domain, arch_post_set_flags
-  for domain_list_inv[wp, DetSchedDomainTime_AI_assms]: "\<lambda>s::det_state. P (domain_list s)"
-  and domain_start_index_inv[wp, DetSchedDomainTime_AI_assms]: "\<lambda>s::det_state. P (domain_start_index s)"
-  (simp: crunch_simps)
-
-crunch arch_finalise_cap
-  for domain_time_inv[wp, DetSchedDomainTime_AI_assms]: "\<lambda>s. P (domain_time s)"
-  and domain_start_index_inv[wp, DetSchedDomainTime_AI_assms]: "\<lambda>s::det_state. P (domain_start_index s)"
-  (wp: hoare_drop_imps mapM_wp subset_refl simp: crunch_simps)
-
-crunch
-  arch_activate_idle_thread, arch_switch_to_thread, arch_switch_to_idle_thread,
-  handle_arch_fault_reply, init_arch_objects,
-  arch_invoke_irq_control, arch_get_sanitise_register_info,
-  prepare_thread_delete, handle_hypervisor_fault, handle_vm_fault,
-  arch_post_modify_registers, arch_post_cap_deletion,
-  arch_invoke_irq_handler, arch_prepare_next_domain, arch_prepare_set_domain, arch_post_set_flags
-  for domain_time_inv[wp, DetSchedDomainTime_AI_assms]: "\<lambda>s::det_state. P (domain_time s)"
+  for domain_fields_invs[wp, DetSchedDomainTime_AI_assms]: "domain_fields P"
   (simp: crunch_simps)
 
 crunch do_machine_op
@@ -50,17 +30,15 @@ declare init_arch_objects_exst[DetSchedDomainTime_AI_assms]
 end
 
 global_interpretation DetSchedDomainTime_AI?: DetSchedDomainTime_AI
-  proof goal_cases
+proof goal_cases
   interpret Arch .
   case 1 show ?case by (unfold_locales; (fact DetSchedDomainTime_AI_assms)?)
-  qed
+qed
 
 context Arch begin arch_global_naming
 
 crunch arch_perform_invocation
-  for domain_time_inv[wp, DetSchedDomainTime_AI_assms]: "\<lambda>s::det_state. P (domain_time s)"
-  and domain_list_inv[wp, DetSchedDomainTime_AI_assms]: "\<lambda>s::det_state. P (domain_list s)"
-  and domain_start_index_inv[wp, DetSchedDomainTime_AI_assms]: "\<lambda>s::det_state. P (domain_start_index s)"
+  for domain_fields_invs[wp, DetSchedDomainTime_AI_assms]: "domain_fields P"
   (wp: crunch_wps check_cap_inv)
 
 lemma timer_tick_valid_domain_time:
@@ -101,9 +79,7 @@ lemma handle_interrupt_valid_domain_time [DetSchedDomainTime_AI_assms]:
   done
 
 crunch handle_reserved_irq, arch_mask_irq_signal, handle_spurious_irq
-  for domain_time_inv [wp, DetSchedDomainTime_AI_assms]: "\<lambda>s. P (domain_time s)"
-  and domain_list_inv [wp, DetSchedDomainTime_AI_assms]: "\<lambda>s. P (domain_list s)"
-  and domain_start_index_inv[wp, DetSchedDomainTime_AI_assms]: "\<lambda>s::det_state. P (domain_start_index s)"
+  for domain_fields_invs[wp, DetSchedDomainTime_AI_assms]: "domain_fields P"
   (wp: crunch_wps mapM_wp subset_refl simp: crunch_simps)
 
 crunch handle_spurious_irq
@@ -112,9 +88,9 @@ crunch handle_spurious_irq
 end
 
 global_interpretation DetSchedDomainTime_AI_2?: DetSchedDomainTime_AI_2
-  proof goal_cases
+proof goal_cases
   interpret Arch .
   case 1 show ?case by (unfold_locales; (fact DetSchedDomainTime_AI_assms)?)
-  qed
+qed
 
 end
